theories/Iris/Model.v
@@ -112,169 +112,180 @@ Next Obligation.
 Qed.
 Canonical IProp.
 
-Module Iris
-  (Import B    : Base)
-  (Import SPEC : Specification B)
-  (Import SEM  : Semantics B SPEC.PROG)
-  (Import PLOG : ProgramLogicOn B SPEC).
+Module IrisPrelims
+    (Import B    : Base)
+    (Import P    : Program B)
+    (Import SpecMixin : ProgSpecMixinOn B P)
+    (Import SEM  : Semantics B P).
 
-Import SmallStepNotations.
+  Import SmallStepNotations.
 
-Section Language.
+  Section Language.
 
-  (* The "expressions" of the LanguageMixin are configurations consisting of a
-     statement and a local variable store. *)
-  Record Conf (Γ : PCtx) τ : Type :=
-    MkConf
-      { conf_stm   : Stm Γ τ;
-        conf_store : CStore Γ
-      }.
-
-  Section TransparentObligations.
-    Local Set Transparent Obligations.
-    Derive NoConfusion for Conf.
-  End TransparentObligations.
-
-  (* The "values" of the LanguageMixin are final configurations consisting of a
-     value and a store. We only keep the store around for technical reasons,
-     essentially to validate of_to_val. *)
-  Section ValConf.
-    Local Set Primitive Projections.
-    Record ValConf (Γ : PCtx) τ : Type :=
-      MkValConf
-        { valconf_val   : Val τ;
-          valconf_store : CStore Γ
+    (* The "expressions" of the LanguageMixin are configurations consisting of a
+       statement and a local variable store. *)
+    Record Conf (Γ : PCtx) τ : Type :=
+      MkConf
+        { conf_stm   : Stm Γ τ;
+          conf_store : CStore Γ
         }.
-  End ValConf.
 
-  Definition of_val {Γ} {τ} (v : ValConf Γ τ) : Conf Γ τ :=
-    match v with
-      MkValConf _ v δ => MkConf (stm_val _ v) δ
-    end.
+    Section TransparentObligations.
+      Local Set Transparent Obligations.
+      Derive NoConfusion for Conf.
+    End TransparentObligations.
 
-  Definition to_val {Γ} {τ} (t : Conf Γ τ) : option (ValConf Γ τ) :=
-    match t with
-    | MkConf (stm_val _ v) δ => Some (MkValConf _ v δ)
-    | _                      => None
-    end.
+    (* The "values" of the LanguageMixin are final configurations consisting of a
+       value and a store. We only keep the store around for technical reasons,
+       essentially to validate of_to_val. *)
+    Section ValConf.
+      Local Set Primitive Projections.
+      Record ValConf (Γ : PCtx) τ : Type :=
+        MkValConf
+          { valconf_val   : Val τ;
+            valconf_store : CStore Γ
+          }.
+    End ValConf.
 
-  Lemma to_of_val {Γ} {τ} (v : ValConf Γ τ) : to_val (of_val v) = Some v.
-  Proof.
-    by destruct v.
-  Qed.
+    Definition of_val {Γ} {τ} (v : ValConf Γ τ) : Conf Γ τ :=
+      match v with
+        MkValConf _ v δ => MkConf (stm_val _ v) δ
+      end.
 
-  Lemma of_to_val {Γ} {τ} (s : Conf Γ τ) v : to_val s = Some v → of_val v = s.
-  Proof.
-    destruct s as [s δ]; destruct s; try done.
-    by intros [= <-].
-  Qed.
+    Definition to_val {Γ} {τ} (t : Conf Γ τ) : option (ValConf Γ τ) :=
+      match t with
+      | MkConf (stm_val _ v) δ => Some (MkValConf _ v δ)
+      | _                      => None
+      end.
 
-  Lemma val_head_stuck_step {τ} {Γ : PCtx} γ1 γ2 μ1 μ2 (δ1 : CStore Γ) δ2 (s1 : Stm Γ τ) s2 :
-    ⟨ γ1, μ1, δ1, s1 ⟩ ---> ⟨ γ2, μ2, δ2, s2 ⟩ -> to_val (MkConf s1 δ1) = None.
-  Proof.
-    by induction 1.
-  Qed.
+    Lemma to_of_val {Γ} {τ} (v : ValConf Γ τ) : to_val (of_val v) = Some v.
+    Proof.
+      by destruct v.
+    Qed.
 
-  Definition observation := Empty_set.
+    Lemma of_to_val {Γ} {τ} (s : Conf Γ τ) v : to_val s = Some v → of_val v = s.
+    Proof.
+      destruct s as [s δ]; destruct s; try done.
+      by intros [= <-].
+    Qed.
 
-  Definition State := prod RegStore Memory.
+    Lemma val_head_stuck_step {τ} {Γ : PCtx} γ1 γ2 μ1 μ2 (δ1 : CStore Γ) δ2 (s1 : Stm Γ τ) s2 :
+      ⟨ γ1, μ1, δ1, s1 ⟩ ---> ⟨ γ2, μ2, δ2, s2 ⟩ -> to_val (MkConf s1 δ1) = None.
+    Proof.
+      by induction 1.
+    Qed.
 
-  Inductive prim_step {Γ τ} : Conf Γ τ -> State -> list Empty_set -> Conf Γ τ -> State -> list (Conf Γ τ) -> Prop :=
-  | mk_prim_step γ1 γ2 μ1 μ2 (δ1 : CStore Γ) (δ2 : CStore Γ) s1 s2 :
-      ⟨ γ1, μ1, δ1, s1 ⟩ ---> ⟨ γ2, μ2, δ2, s2 ⟩ ->
-      prim_step (MkConf s1 δ1) (γ1 , μ1) nil (MkConf s2 δ2) (γ2 , μ2) nil
-  .
+    Definition observation := Empty_set.
 
-  Lemma val_head_stuck {Γ τ} (e1 : Conf Γ τ) s1 ls e2 s2 {ks} : prim_step e1 s1 ls e2 s2 ks → to_val e1 = None.
-  Proof.
-    induction 1.
-    by eapply val_head_stuck_step.
-  Qed.
+    Definition State := prod RegStore Memory.
 
-  Lemma microsail_lang_mixin Γ τ : LanguageMixin of_val to_val (@prim_step Γ τ).
-  Proof. split; eauto using to_of_val, of_to_val, val_head_stuck. Qed.
+    Inductive prim_step {Γ τ} : Conf Γ τ -> State -> list Empty_set -> Conf Γ τ -> State -> list (Conf Γ τ) -> Prop :=
+    | mk_prim_step γ1 γ2 μ1 μ2 (δ1 : CStore Γ) (δ2 : CStore Γ) s1 s2 :
+        ⟨ γ1, μ1, δ1, s1 ⟩ ---> ⟨ γ2, μ2, δ2, s2 ⟩ ->
+        prim_step (MkConf s1 δ1) (γ1 , μ1) nil (MkConf s2 δ2) (γ2 , μ2) nil
+    .
 
-  Canonical Structure microsail_lang Γ τ : language := Language (microsail_lang_mixin Γ τ).
+    Lemma val_head_stuck {Γ τ} (e1 : Conf Γ τ) s1 ls e2 s2 {ks} : prim_step e1 s1 ls e2 s2 ks → to_val e1 = None.
+    Proof.
+      induction 1.
+      by eapply val_head_stuck_step.
+    Qed.
 
-  Global Instance intoVal_valconf {Γ τ δ v} : IntoVal (MkConf (Γ := Γ) (τ := τ) (stm_val _ v) δ) (MkValConf _ v δ).
-    intros; eapply of_to_val; by cbn.
-  Defined.
+    Lemma microsail_lang_mixin Γ τ : LanguageMixin of_val to_val (@prim_step Γ τ).
+    Proof. split; eauto using to_of_val, of_to_val, val_head_stuck. Qed.
 
-End Language.
+    Canonical Structure microsail_lang Γ τ : language := Language (microsail_lang_mixin Γ τ).
 
-Section Registers.
+    Global Instance intoVal_valconf {Γ τ δ v} : IntoVal (MkConf (Γ := Γ) (τ := τ) (stm_val _ v) δ) (MkValConf _ v δ).
+      intros; eapply of_to_val; by cbn.
+    Defined.
 
-  Definition SomeReg : Type := sigT 𝑹𝑬𝑮.
-  Definition SomeVal : Type := sigT Val.
+  End Language.
 
-  Global Instance eqDec_SomeReg : EqDec SomeReg := 𝑹𝑬𝑮_eq_dec.
-  Global Instance countable_SomeReg : countable.Countable SomeReg := finite.finite_countable.
+  Section Registers.
 
-  Global Instance eqDec_SomeVal : EqDec SomeVal.
-  Proof.
-    intros [τ1 v1] [τ2 v2].
-    destruct (Ty_eq_dec τ1 τ2).
-    - subst.
-      destruct (Val_eqb_spec _ v1 v2).
-      + left. congruence.
-      + right. intros H.
-        Local Set Equations With UIP.
+    Definition SomeReg : Type := sigT 𝑹𝑬𝑮.
+    Definition SomeVal : Type := sigT Val.
+
+    Global Instance eqDec_SomeReg : EqDec SomeReg := 𝑹𝑬𝑮_eq_dec.
+    Global Instance countable_SomeReg : countable.Countable SomeReg := finite.finite_countable.
+
+    Global Instance eqDec_SomeVal : EqDec SomeVal.
+    Proof.
+      intros [τ1 v1] [τ2 v2].
+      destruct (Ty_eq_dec τ1 τ2).
+      - subst.
+        destruct (Val_eqb_spec _ v1 v2).
+        + left. congruence.
+        + right. intros H.
+          Local Set Equations With UIP.
+          by dependent elimination H.
+      - right. intros H.
         by dependent elimination H.
-    - right. intros H.
-      by dependent elimination H.
-  Qed.
+    Qed.
 
-  Definition regUR := authR (gmapUR SomeReg (exclR (leibnizO SomeVal))).
-  (* Definition regUR' : cmra := *)
-  (*   authR (discrete_funUR (A := SomeReg) *)
-  (*            (fun '(existT σ r) => excl_auth.excl_authUR (leibnizO (Val σ)))). *)
+    Definition regUR := authR (gmapUR SomeReg (exclR (leibnizO SomeVal))).
+    (* Definition regUR' : cmra := *)
+    (*   authR (discrete_funUR (A := SomeReg) *)
+    (*            (fun '(existT σ r) => excl_auth.excl_authUR (leibnizO (Val σ)))). *)
 
-  Class sailRegGS Σ := SailRegGS {
-                          (* ghost variable for tracking state of registers *)
-                          reg_inG :> inG Σ regUR;
-                          reg_gv_name : gname;
-                        }.
+    Class sailRegGS Σ := SailRegGS {
+                            (* ghost variable for tracking state of registers *)
+                            reg_inG :> inG Σ regUR;
+                            reg_gv_name : gname;
+                          }.
 
-  Definition reg_pointsTo `{sailRegGS Σ} {τ} (r : 𝑹𝑬𝑮 τ) (v : Val τ) : iProp Σ :=
-    own reg_gv_name (◯ {[ existT _ r := Excl (existT _ v) ]}).
+    Definition reg_pointsTo `{sailRegGS Σ} {τ} (r : 𝑹𝑬𝑮 τ) (v : Val τ) : iProp Σ :=
+      own reg_gv_name (◯ {[ existT _ r := Excl (existT _ v) ]}).
 
-  Definition regs_inv `{sailRegGS Σ} (regstore : RegStore) : iProp Σ :=
-    (∃ regsmap,
-        own reg_gv_name (● regsmap) ∗
-        ⌜ map_Forall (K := SomeReg) (A := excl SomeVal) (fun reg v => match reg with | existT _ reg => Excl (existT _ (read_register regstore reg)) = v end ) regsmap ⌝
-    )%I.
+    Definition regs_inv `{sailRegGS Σ} (regstore : RegStore) : iProp Σ :=
+      (∃ regsmap,
+          own reg_gv_name (● regsmap) ∗
+          ⌜ map_Forall (K := SomeReg) (A := excl SomeVal) (fun reg v => match reg with | existT _ reg => Excl (existT _ (read_register regstore reg)) = v end ) regsmap ⌝
+      )%I.
 
-End Registers.
+  End Registers.
+End IrisPrelims.
 
-Module Type IrisHeapKit.
+
+Module Type IrisParameters
+  (Import B    : Base)
+  (Import P : Program B)
+  (Import SIG : ProgramLogicSignature B)
+  (Import SEM  : Semantics B P).
+  Include IrisPrelims B P SIG SEM.
   Parameter memGpreS : gFunctors -> Set.
   Parameter memGS : gFunctors -> Set.
   Parameter memΣ : gFunctors.
-
   Parameter memΣ_GpreS : forall {Σ}, subG memΣ Σ -> memGpreS Σ.
-
   Parameter mem_inv : forall {Σ}, memGS Σ -> Memory -> iProp Σ.
   Parameter mem_res : forall {Σ}, memGS Σ -> Memory -> iProp Σ.
 
-  (* Definition mem_inv `{sailG Σ} (μ : Z -> option Z) : iProp Σ := *)
-  (*   (∃ memmap, gen_heap_ctx memmap ∗ *)
-  (*      ⌜ map_Forall (fun (a : Z) v => μ a = Some v) memmap ⌝ *)
-  (*   )%I. *)
+    (* Definition mem_inv `{sailG Σ} (μ : Z -> option Z) : iProp Σ := *)
+    (*   (∃ memmap, gen_heap_ctx memmap ∗ *)
+    (*      ⌜ map_Forall (fun (a : Z) v => μ a = Some v) memmap ⌝ *)
+    (*   )%I. *)
 
   Parameter mem_inv_init : forall Σ (μ : Memory), memGpreS Σ ->
-    ⊢ |==> ∃ mG : memGS Σ, (mem_inv mG μ ∗ mem_res mG μ)%I.
+                                         ⊢ |==> ∃ mG : memGS Σ, (mem_inv mG μ ∗ mem_res mG μ)%I.
 
   Parameter luser_inst : forall `{sRG : sailRegGS Σ} `{invGS Σ} (mG : memGS Σ) (p : 𝑯) (ts : Env Val (𝑯_Ty p)), iProp Σ.
   Parameter lduplicate_inst : forall `{sRG : sailRegGS Σ} `{invGS Σ} (mG : memGS Σ) (p : 𝑯) (ts : Env Val (𝑯_Ty p)),
-      is_duplicable p = true -> bi_entails (luser_inst mG ts) (luser_inst mG ts ∗ luser_inst mG ts).
+      is_duplicable p = true -> bi_entails (luser_inst (sRG := sRG) mG ts) (luser_inst (sRG := sRG) mG ts ∗ luser_inst (sRG := sRG) mG ts).
+End IrisParameters.
 
-End IrisHeapKit.
 
-Module IrisInstance (Import K : IrisHeapKit).
+(*
+ * The following module defines the Iris model depending solely on the ProgramLogicSignature, not only the Specification.
+ * This allows us to use multiple different specifications with the same Iris model, so that the resulting triples can be combined.
+ * This is important particularly in the RiscvPmp.BlockVerification proofs.
+ *)
+Module Type IrisInstance
+  (Import B    : Base)
+  (Import SIG : ProgramLogicSignature B)
+  (Import SEM  : Semantics B SIG.PROG)
+  (Import IParam  : IrisParameters B SIG.PROG SIG SEM).
 Section Soundness.
-
-  Existing Class memGpreS.
-  Existing Class memGS.
 
   Class sailGpreS Σ := SailGpreS { (* resources for the implementation side *)
                        sailGpresS_invGpreS :> invGpreS Σ; (* for fancy updates, invariants... *)
@@ -302,12 +313,12 @@ Section Soundness.
                                                                                 }.
   Global Opaque iris_invGS.
 
-  Context {Σ} {sG : sailGS Σ}.
+  Context `{sG : sailGS Σ}.
 
   Global Instance PredicateDefIProp : PredicateDef (IProp Σ) :=
     {| lptsreg σ r v        := reg_pointsTo r v;
        luser p ts           := luser_inst sailGS_memGS ts;
-       lduplicate p ts Hdup := lduplicate_inst sailGS_memGS ts Hdup
+       lduplicate p ts Hdup := lduplicate_inst (sRG := sailGS_sailRegGS) sailGS_memGS ts Hdup
     |}.
 
   Lemma reg_valid regstore {τ} (r : 𝑹𝑬𝑮 τ) (v : Val τ) :
@@ -380,7 +391,7 @@ Section Soundness.
     iApply (regs_inv_update H); iFrame.
   Qed.
 
-  Lemma rule_stm_read_register {Γ τ} (r : 𝑹𝑬𝑮 τ) (v : Val τ) {δ : CStore Γ} :
+  Lemma iris_rule_stm_read_register_wp {Γ τ} (r : 𝑹𝑬𝑮 τ) (v : Val τ) {δ : CStore Γ} :
     ⊢ (lptsreg r v -∗
                     WP (MkConf (stm_read_register r) δ) ?{{ w, lptsreg r v ∗ ⌜ w = MkValConf _ v δ ⌝ }}
       )%I.
@@ -402,7 +413,7 @@ Section Soundness.
     by iApply wp_value.
   Qed.
 
-  Lemma rule_stm_write_register {Γ} {τ} (r : 𝑹𝑬𝑮 τ) (δ : CStore Γ) (v : Val τ) e :
+  Lemma iris_rule_stm_write_register_wp {Γ} {τ} (r : 𝑹𝑬𝑮 τ) (δ : CStore Γ) (v : Val τ) e :
     ⊢ (reg_pointsTo r v -∗
                     WP (MkConf (stm_write_register r e) δ : expr (microsail_lang Γ τ)) ?{{ w, reg_pointsTo r (eval e δ) ∗ bi_pure (w = MkValConf _ (eval e δ) δ) }}
     )%I.
@@ -1028,7 +1039,7 @@ Section Soundness.
         ⊢ (semTriple δ (lptsreg r v) (stm_read_register r) (fun v' δ' => ⌜ δ' = δ ⌝ ∧ ⌜ v' = v ⌝ ∧ lptsreg r v))%I.
   Proof.
     iIntros "Hreg".
-    iApply wp_mono; [| iApply (rule_stm_read_register with "Hreg") ].
+    iApply wp_mono; [| iApply (iris_rule_stm_read_register_wp with "Hreg") ].
     iIntros ([δ' v']) "[Hreg %]".
     inversion H.
     by iFrame.
@@ -1042,7 +1053,7 @@ Section Soundness.
                   (fun v' δ' => ⌜δ' = δ⌝ ∧ ⌜v' = eval w δ⌝ ∧ lptsreg r v')%I.
   Proof.
     iIntros "Hreg".
-    iApply wp_mono; [|iApply (rule_stm_write_register with "Hreg")].
+    iApply wp_mono; [|iApply (iris_rule_stm_write_register_wp with "Hreg")].
     iIntros (v') "[Hreg %]".
     rewrite H.
     by iFrame.
@@ -1194,60 +1205,6 @@ Section Soundness.
       iApply wp_compat_fail.
   Qed.
 
-  Lemma iris_rule_stm_call_forwards {Γ} (δ : CStore Γ)
-        {Δ σ} (f : 𝑭 Δ σ) (c : SepContract Δ σ) (es : NamedEnv (Exp Γ) Δ)
-        (P : iProp Σ)
-        (Q : Val σ -> iProp Σ) :
-        CEnv f = Some c ->
-        CTriple (evals es δ) P Q c ->
-        (⊢ ▷ ValidContractEnvSem CEnv -∗
-           semTriple δ P (stm_call f es) (fun v δ' => Q v ∧ bi_pure (δ = δ')))%I.
-  Proof.
-    iIntros (ceq ctrip) "cenv P".
-    rewrite wp_unfold. cbn.
-    iIntros ([regs μ] ns ks1 ks nt) "Hregs".
-    iMod (fupd_mask_subseteq empty) as "Hclose"; first set_solver.
-    iModIntro.
-    iSplitR; [trivial|].
-    iIntros (e2 [regs2 μ2] efs) "%".
-    unfold language.prim_step in H; cbn in H.
-    dependent elimination H.
-    dependent elimination s.
-    iModIntro. iModIntro. iModIntro.
-    iMod "Hclose" as "_".
-    iModIntro.
-    iFrame.
-    iSplitL; [|trivial].
-    destruct ctrip.
-    iPoseProof (H0 with "P") as "[fr req]".
-    iApply wp_compat_call_frame.
-    rewrite H.
-    iApply (wp_mono _ _ _ (fun v => frame ∗ match v with
-                                            | MkValConf _ v _ => interpret_assertion ens (env.snoc ι (result∷σ) v)
-                                            end)%I).
-    - intros [v δ']; cbn.
-      iIntros "[fr ens]".
-      iSplitL; [|trivial].
-      iApply (H1 v).
-      by iFrame.
-    - iSpecialize ("cenv" $! _ _ f0).
-      rewrite ceq.
-      iSpecialize ("cenv" $! ι with "req").
-      iApply wp_frame_l.
-      by iFrame.
-  Qed.
-
-  Lemma iris_rule_stm_call_frame {Γ} (δ : CStore Γ)
-        (Δ : PCtx) (δΔ : CStore Δ) (τ : Ty) (s : Stm Δ τ)
-        (P : iProp Σ) (Q : Val τ -> CStore Γ -> iProp Σ) :
-        ⊢ (semTriple δΔ P s (fun v _ => Q v δ) -∗
-           semTriple δ P (stm_call_frame δΔ s) Q)%I.
-  Proof.
-    iIntros "trips P".
-    iSpecialize ("trips" with "P").
-    by iApply wp_compat_call_frame.
-  Qed.
-
   Lemma iris_rule_stm_bind {Γ} (δ : CStore Γ)
         {σ τ : Ty} (s : Stm Γ σ) (k : Val σ -> Stm Γ τ)
         (P : iProp Σ) (Q : Val σ -> CStore Γ -> iProp Σ)
@@ -1339,44 +1296,6 @@ Section Soundness.
     iApply (iris_rule_stm_call_inline_later with "Hdef").
   Qed.
 
-  Definition ForeignSem :=
-    ∀ (Γ : NCtx 𝑿 Ty) (τ : Ty)
-      (Δ : NCtx 𝑿 Ty) f (es : NamedEnv (Exp Γ) Δ) (δ : CStore Γ),
-      match CEnvEx f with
-      | MkSepContract _ _ Σ' θΔ req result ens =>
-        forall (ι : Valuation Σ'),
-        evals es δ = inst θΔ ι ->
-        ⊢ semTriple δ (interpret_assertion req ι) (stm_foreign f es)
-          (fun v δ' => interpret_assertion ens (env.snoc ι (result∷τ) v) ∗ bi_pure (δ' = δ))
-      end.
-
-  Lemma iris_rule_stm_foreign
-    {Γ} (δ : CStore Γ) {τ} {Δ} (f : 𝑭𝑿 Δ τ) (es : NamedEnv (Exp Γ) Δ)
-    (P : iProp Σ) (Q : Val τ -> CStore Γ -> iProp Σ) :
-    ForeignSem ->
-    CTriple (evals es δ) P (λ v : Val τ, Q v δ) (CEnvEx f) ->
-    ⊢ semTriple δ P (stm_foreign f es) Q.
-  Proof.
-    iIntros (extSem ctrip).
-    specialize (extSem _ _ _ f es δ).
-    revert ctrip extSem.
-    generalize (CEnvEx f) as contractF.
-    intros contractF ctrip extSem.
-    destruct ctrip; cbn in extSem.
-    iIntros "P".
-    iPoseProof (H0 with "P") as "[frm pre]".
-    iApply (wp_mono _ _ _ (fun v => frame ∗ match v with MkValConf _ v δ' => interpret_assertion (HProp := IProp Σ) ens (env.snoc ι (result∷τ) v) ∗ bi_pure (δ' = δ) end)%I).
-    - intros v.
-      destruct v.
-      iIntros "[frame [pre %]]".
-      subst.
-      iApply H1.
-      by iFrame.
-    - iApply wp_frame_l.
-      iFrame.
-      by iApply (extSem ι H).
-  Qed.
-
   Definition ValidLemma {Δ} (lem : Lemma Δ) : Prop :=
     match lem with
       {| lemma_logic_variables := Σ;
@@ -1388,44 +1307,6 @@ Section Soundness.
         ⊢ interpret_assertion req ι -∗
           interpret_assertion ens ι
     end.
-
-  Definition LemmaSem : Prop :=
-    forall (Δ : NCtx 𝑿 Ty) (l : 𝑳 Δ),
-      ValidLemma (LEnv l).
-
-  Lemma iris_rule_stm_lemmak
-    {Γ} (δ : CStore Γ) {τ} {Δ} (l : 𝑳 Δ) (es : NamedEnv (Exp Γ) Δ) (k : Stm Γ τ)
-    (P Q : iProp Σ) (R : Val τ -> CStore Γ -> iProp Σ) :
-    LemmaSem ->
-    LTriple (evals es δ) P Q (LEnv l) ->
-    ⊢ semTriple δ Q k R -∗
-      semTriple δ P (stm_lemmak l es k) R.
-  Proof.
-    iIntros (lemSem ltrip).
-    specialize (lemSem _ l).
-    revert ltrip lemSem.
-    generalize (LEnv l) as contractL.
-    intros contractL ltrip lemSem.
-    dependent elimination ltrip; cbn in lemSem.
-    specialize (lemSem ι).
-    iIntros "tripk P".
-    rewrite wp_unfold. cbn.
-    iIntros (σ ns ks1 ks nt) "Hregs".
-    iMod (fupd_mask_subseteq empty) as "Hclose"; first set_solver.
-    iModIntro. iSplitR; [trivial|].
-    iIntros (e3 σ2 efs) "%".
-    dependent elimination H.
-    dependent elimination s.
-    iModIntro. iModIntro. iModIntro.
-    iMod "Hclose" as "_".
-    iModIntro; iFrame.
-    iSplitL; [|trivial].
-    iApply "tripk".
-    iApply l1.
-    iPoseProof (l0 with "P") as "[frm pre]".
-    iFrame.
-    by iApply lemSem.
-  Qed.
 
   Lemma iris_rule_stm_debugk
     {Γ τ} (δ : CStore Γ) (k : Stm Γ τ)
@@ -1484,69 +1365,11 @@ Section Soundness.
       now iApply wp_compat_fail.
   Qed.
 
-  Lemma sound_stm {Γ} {τ} (s : Stm Γ τ) {δ : CStore Γ}:
-    forall (PRE : iProp Σ) (POST : Val τ -> CStore Γ -> iProp Σ),
-      ForeignSem ->
-      LemmaSem ->
-      ⦃ PRE ⦄ s ; δ ⦃ POST ⦄ ->
-      ⊢ (□ ▷ ValidContractEnvSem CEnv -∗
-          semTriple δ PRE s POST)%I.
-  Proof.
-    iIntros (PRE POST extSem lemSem triple) "#vcenv".
-    iInduction triple as [x|x|x|x|x|x|x|x|x|x|x|x|x|x|x|x|x|x|x|x|x|x|x|x|x|x|x|x|x|x|x] "trips".
-    - by iApply iris_rule_consequence.
-    - by iApply iris_rule_frame.
-    - by iApply iris_rule_pull.
-    - by iApply iris_rule_exist.
-    - iApply iris_rule_stm_val.
-      by iApply H.
-    - iApply iris_rule_stm_exp.
-      by iApply H.
-    - by iApply iris_rule_stm_let.
-    - by iApply iris_rule_stm_block.
-    - by iApply iris_rule_stm_if.
-    - by iApply iris_rule_stm_seq.
-    - by iApply iris_rule_stm_assertk.
-    - by iApply iris_rule_stm_fail.
-    - by iApply iris_rule_stm_match_list.
-    - by iApply iris_rule_stm_match_sum.
-    - by iApply iris_rule_stm_match_prod.
-    - by iApply iris_rule_stm_match_enum.
-    - by iApply iris_rule_stm_match_tuple.
-    - by iApply iris_rule_stm_match_union.
-    - by iApply iris_rule_stm_match_record.
-    - by iApply iris_rule_stm_match_bvec.
-    - by iApply iris_rule_stm_read_register.
-    - by iApply iris_rule_stm_write_register.
-    - by iApply iris_rule_stm_assign_backwards.
-    - by iApply iris_rule_stm_assign_forwards.
-    - by iApply iris_rule_stm_call_forwards.
-    - by iApply iris_rule_stm_call_inline.
-    - by iApply iris_rule_stm_call_frame.
-    - by iApply iris_rule_stm_foreign.
-    - by iApply iris_rule_stm_lemmak.
-    - by iApply iris_rule_stm_bind.
-    - by iApply iris_rule_stm_debugk.
-  Qed.
-
-  Lemma sound :
-    ForeignSem -> LemmaSem -> ValidContractCEnv ->
-    ⊢ ValidContractEnvSem CEnv.
-  Proof.
-    intros extSem lemSem vcenv.
-    iLöb as "IH".
-    iIntros (σs σ f).
-    specialize (vcenv σs σ f).
-    destruct (CEnv f) as [[]|];[|trivial].
-    specialize (vcenv _ eq_refl).
-    iIntros (ι).
-    iApply (sound_stm extSem lemSem); [|trivial].
-    apply (vcenv ι).
-  Qed.
-
 End Soundness.
 
 Section Adequacy.
+
+  Import SmallStepNotations.
 
   Definition sailΣ : gFunctors := #[ memΣ ; invΣ ; GFunctor regUR].
 
@@ -1703,4 +1526,211 @@ Section Adequacy.
   Qed.
 End Adequacy.
 End IrisInstance.
-End Iris.
+
+(*
+ * The following module defines the parts of the Iris model that must depend on the Specification, not just on the ProgramLogicSignature.
+ * This is kept to a minimum (see comment for the IrisInstance module).
+ *)
+Module IrisInstanceWithContracts
+  (Import B    : Base)
+  (Import SIG  : ProgramLogicSignature B)
+  (Import SPEC  : Specification B SIG)
+  (Import SEM  : Semantics B SIG.PROG)
+  (Import IP   : IrisParameters B SIG.PROG SIG SEM)
+  (Import II   : IrisInstance B SIG SEM IP)
+  (Import PLOG : ProgramLogicOn B SIG SPEC).
+
+  Context `{sailGS Σ}.
+
+  Definition ForeignSem :=
+    ∀ (Γ : NCtx 𝑿 Ty) (τ : Ty)
+      (Δ : NCtx 𝑿 Ty) f (es : NamedEnv (Exp Γ) Δ) (δ : CStore Γ),
+      match CEnvEx f with
+      | MkSepContract _ _ Σ' θΔ req result ens =>
+        forall (ι : Valuation Σ'),
+        evals es δ = inst θΔ ι ->
+        ⊢ semTriple δ (interpret_assertion req ι) (stm_foreign f es)
+          (fun v δ' => interpret_assertion ens (env.snoc ι (result∷τ) v) ∗ bi_pure (δ' = δ))
+      end.
+
+  Definition LemmaSem : Prop :=
+    forall (Δ : NCtx 𝑿 Ty) (l : 𝑳 Δ),
+      ValidLemma (LEnv l).
+
+  Lemma iris_rule_stm_call_forwards `{sG : sailGS Σ} {Γ} (δ : CStore Γ)
+        {Δ σ} (f : 𝑭 Δ σ) (c : SepContract Δ σ) (es : NamedEnv (Exp Γ) Δ)
+        (P : iProp Σ)
+        (Q : Val σ -> iProp Σ) :
+        CEnv f = Some c ->
+        CTriple (evals es δ) P Q c ->
+        (⊢ ▷ ValidContractEnvSem CEnv -∗
+           semTriple δ P (stm_call f es) (fun v δ' => Q v ∧ bi_pure (δ = δ')))%I.
+  Proof.
+    iIntros (ceq ctrip) "cenv P".
+    rewrite wp_unfold. cbn.
+    iIntros ([regs μ] ns ks1 ks nt) "Hregs".
+    iMod (fupd_mask_subseteq empty) as "Hclose"; first set_solver.
+    iModIntro.
+    iSplitR; [trivial|].
+    iIntros (e2 [regs2 μ2] efs) "%".
+    unfold language.prim_step in H0; cbn in H0.
+    dependent elimination H0.
+    dependent elimination s.
+    iModIntro. iModIntro. iModIntro.
+    iMod "Hclose" as "_".
+    iModIntro.
+    iFrame.
+    iSplitL; [|trivial].
+    destruct ctrip.
+    iPoseProof (H1 with "P") as "[fr req]".
+    iApply wp_compat_call_frame.
+    rewrite H0.
+    iApply (wp_mono _ _ _ (fun v => frame ∗ match v with
+                                            | MkValConf _ v _ => interpret_assertion ens (env.snoc ι (result∷σ) v)
+                                            end)%I).
+    - intros [v δ']; cbn.
+      iIntros "[fr ens]".
+      iSplitL; [|trivial].
+      iApply (H2 v).
+      by iFrame.
+    - iSpecialize ("cenv" $! _ _ f0).
+      rewrite ceq.
+      iSpecialize ("cenv" $! ι with "req").
+      iApply wp_frame_l.
+      by iFrame.
+  Qed.
+
+  Lemma iris_rule_stm_call_frame {Γ} (δ : CStore Γ)
+        (Δ : PCtx) (δΔ : CStore Δ) (τ : Ty) (s : Stm Δ τ)
+        (P : iProp Σ) (Q : Val τ -> CStore Γ -> iProp Σ) :
+        ⊢ (semTriple δΔ P s (fun v _ => Q v δ) -∗
+           semTriple δ P (stm_call_frame δΔ s) Q)%I.
+  Proof.
+    iIntros "trips P".
+    iSpecialize ("trips" with "P").
+    by iApply wp_compat_call_frame.
+  Qed.
+
+  Lemma iris_rule_stm_foreign
+    {Γ} (δ : CStore Γ) {τ} {Δ} (f : 𝑭𝑿 Δ τ) (es : NamedEnv (Exp Γ) Δ)
+    (P : iProp Σ) (Q : Val τ -> CStore Γ -> iProp Σ) :
+    ForeignSem ->
+    CTriple (evals es δ) P (λ v : Val τ, Q v δ) (CEnvEx f) ->
+    ⊢ semTriple δ P (stm_foreign f es) Q.
+  Proof.
+    iIntros (extSem ctrip).
+    specialize (extSem _ _ _ f es δ).
+    revert ctrip extSem.
+    generalize (CEnvEx f) as contractF.
+    intros contractF ctrip extSem.
+    destruct ctrip; cbn in extSem.
+    iIntros "P".
+    iPoseProof (H1 with "P") as "[frm pre]".
+    iApply (wp_mono _ _ _ (fun v => frame ∗ match v with MkValConf _ v δ' => interpret_assertion (HProp := IProp Σ) ens (env.snoc ι (result∷τ) v) ∗ bi_pure (δ' = δ) end)%I).
+    - intros v.
+      destruct v.
+      iIntros "[frame [pre %]]".
+      subst.
+      iApply H2.
+      by iFrame.
+    - iApply wp_frame_l.
+      iFrame.
+      by iApply (extSem ι H0).
+  Qed.
+
+  Lemma iris_rule_stm_lemmak
+    {Γ} (δ : CStore Γ) {τ} {Δ} (l : 𝑳 Δ) (es : NamedEnv (Exp Γ) Δ) (k : Stm Γ τ)
+    (P Q : iProp Σ) (R : Val τ -> CStore Γ -> iProp Σ) :
+    LemmaSem ->
+    LTriple (evals es δ) P Q (LEnv l) ->
+    ⊢ semTriple δ Q k R -∗
+      semTriple δ P (stm_lemmak l es k) R.
+  Proof.
+    iIntros (lemSem ltrip).
+    specialize (lemSem _ l).
+    revert ltrip lemSem.
+    generalize (LEnv l) as contractL.
+    intros contractL ltrip lemSem.
+    dependent elimination ltrip; cbn in lemSem.
+    specialize (lemSem ι).
+    iIntros "tripk P".
+    rewrite wp_unfold. cbn.
+    iIntros (σ ns ks1 ks nt) "Hregs".
+    iMod (fupd_mask_subseteq empty) as "Hclose"; first set_solver.
+    iModIntro. iSplitR; [trivial|].
+    iIntros (e3 σ2 efs) "%".
+    dependent elimination H0.
+    dependent elimination s.
+    iModIntro. iModIntro. iModIntro.
+    iMod "Hclose" as "_".
+    iModIntro; iFrame.
+    iSplitL; [|trivial].
+    iApply "tripk".
+    iApply l1.
+    iPoseProof (l0 with "P") as "[frm pre]".
+    iFrame.
+    by iApply lemSem.
+  Qed.
+
+  Lemma sound_stm
+    {Γ} {τ} (s : Stm Γ τ) {δ : CStore Γ}:
+    forall (PRE : iProp Σ) (POST : Val τ -> CStore Γ -> iProp Σ),
+      ForeignSem ->
+      LemmaSem ->
+      ⦃ PRE ⦄ s ; δ ⦃ POST ⦄ ->
+      ⊢ (□ ▷ ValidContractEnvSem CEnv -∗
+          semTriple δ PRE s POST)%I.
+  Proof.
+    iIntros (PRE POST extSem lemSem triple) "#vcenv".
+    iInduction triple as [x|x|x|x|x|x|x|x|x|x|x|x|x|x|x|x|x|x|x|x|x|x|x|x|x|x|x|x|x|x|x] "trips".
+    - by iApply iris_rule_consequence.
+    - by iApply iris_rule_frame.
+    - by iApply iris_rule_pull.
+    - by iApply iris_rule_exist.
+    - iApply iris_rule_stm_val.
+      by iApply H0.
+    - iApply iris_rule_stm_exp.
+      by iApply H0.
+    - by iApply iris_rule_stm_let.
+    - by iApply iris_rule_stm_block.
+    - by iApply iris_rule_stm_if.
+    - by iApply iris_rule_stm_seq.
+    - by iApply iris_rule_stm_assertk.
+    - by iApply iris_rule_stm_fail.
+    - by iApply iris_rule_stm_match_list.
+    - by iApply iris_rule_stm_match_sum.
+    - by iApply iris_rule_stm_match_prod.
+    - by iApply iris_rule_stm_match_enum.
+    - by iApply iris_rule_stm_match_tuple.
+    - by iApply iris_rule_stm_match_union.
+    - by iApply iris_rule_stm_match_record.
+    - by iApply iris_rule_stm_match_bvec.
+    - by iApply iris_rule_stm_read_register.
+    - by iApply iris_rule_stm_write_register.
+    - by iApply iris_rule_stm_assign_backwards.
+    - by iApply iris_rule_stm_assign_forwards.
+    - by iApply iris_rule_stm_call_forwards.
+    - by iApply iris_rule_stm_call_inline.
+    - by iApply iris_rule_stm_call_frame.
+    - by iApply iris_rule_stm_foreign.
+    - by iApply iris_rule_stm_lemmak.
+    - by iApply iris_rule_stm_bind.
+    - by iApply iris_rule_stm_debugk.
+  Qed.
+
+  Lemma sound :
+    ForeignSem -> LemmaSem -> ValidContractCEnv ->
+    ⊢ ValidContractEnvSem CEnv.
+  Proof.
+    intros extSem lemSem vcenv.
+    iLöb as "IH".
+    iIntros (σs σ f).
+    specialize (vcenv σs σ f).
+    destruct (CEnv f) as [[]|];[|trivial].
+    specialize (vcenv _ eq_refl).
+    iIntros (ι).
+    iApply (sound_stm extSem lemSem); [|trivial].
+    apply (vcenv ι).
+  Qed.
+
+End IrisInstanceWithContracts.
